refine: make ghost_relation_wrapper projections generic
Use the _2 approach to make a ghost_relation_wrapper abbreviation that
exposes to generic proofs the fields that ghost_relation can depend on.
This allows generic proofs to automatically simplify most
appearances of ghost_relation_wrapper without additional lemmas.

Signed-off-by: Corey Lewis <corey.lewis@proofcraft.systems>

proof/refine/ARM_HYP/ArchStateRelation.thy
@@ -159,21 +159,21 @@ definition
    | _ \<Rightarrow> True"
 
 definition ghost_relation ::
-  "Structures_A.kheap \<Rightarrow> (word32 \<rightharpoonup> vmpage_size) \<Rightarrow> (word32 \<rightharpoonup> nat) \<Rightarrow> bool" where
+  "kheap \<Rightarrow> (machine_word \<rightharpoonup> vmpage_size) \<Rightarrow> (machine_word \<rightharpoonup> nat) \<Rightarrow> bool" where
   "ghost_relation h ups cns \<equiv>
-   (\<forall>a sz. (\<exists>dev. h a = Some (ArchObj (DataPage dev sz))) \<longleftrightarrow> ups a = Some sz) \<and>
-   (\<forall>a n. (\<exists>cs. h a = Some (CNode n cs) \<and> well_formed_cnode_n n cs) \<longleftrightarrow>
-          cns a = Some n)"
+     (\<forall>a sz. (\<exists>dev. h a = Some (ArchObj (DataPage dev sz))) \<longleftrightarrow> ups a = Some sz) \<and>
+     (\<forall>a n. (\<exists>cs. h a = Some (CNode n cs) \<and> well_formed_cnode_n n cs) \<longleftrightarrow> cns a = Some n)"
 
-(* FIXME arch-split: provided only so that ghost_relation can be used within generic definition
+(* provided only so that ghost_relation can be used within generic definition
    of state_relation (since arch_state_relation doesn't have access to kheap, and
    gsPTTypes on AARCH64 isn't generic) *)
-definition ghost_relation_wrapper :: "det_state \<Rightarrow> kernel_state \<Rightarrow> bool" where
-  "ghost_relation_wrapper s s' \<equiv>
-     ghost_relation (kheap s) (gsUserPages s') (gsCNodes s')"
+definition ghost_relation_wrapper_2 ::
+  "kheap \<Rightarrow> (machine_word \<rightharpoonup> vmpage_size) \<Rightarrow> (machine_word \<rightharpoonup> nat) \<Rightarrow> Arch.kernel_state \<Rightarrow> bool"
+  where
+  "ghost_relation_wrapper_2 h ups cns as \<equiv> ghost_relation h ups cns"
 
 (* inside Arch locale, we have no need for the wrapper *)
-lemmas [simp] = ghost_relation_wrapper_def
+lemmas ghost_relation_wrapper_def[simp] = ghost_relation_wrapper_2_def
 
 definition arch_state_relation :: "(arch_state \<times> ARM_HYP_H.kernel_state) set" where
   "arch_state_relation \<equiv> {(s, s') .
